CSE checkpoint

examples/ghc/theories/TrieMap.v
@@ -1,14 +1,30 @@
+From Coq Require Import ssreflect ssrbool ssrfun.
+From mathcomp Require Import eqtype.
+Set Bullet Behavior "Strict Subproofs".
+
+Generalizable All Variables.
+
 Require Import GHC.Base.     Import GHC.Base.Notations.
 Require Import Data.Functor. Import Data.Functor.Notations.
+Require Import Data.Maybe.
 
 Require Import TrieMap.
 
 Require UniqDFM.
+Require Core.
 
-From Coq Require Import ssreflect ssrbool ssrfun.
-Set Bullet Behavior "Strict Subproofs".
+(** * Don't unfold TrieMap operations. *)
 
-Generalizable All Variables.
+Arguments Key      : simpl never.
+Arguments alterTM  : simpl never.
+Arguments emptyTM  : simpl never.
+Arguments foldTM   : simpl never.
+Arguments lookupTM : simpl never.
+Arguments mapTM    : simpl never.
+Arguments insertTM : simpl never.
+Arguments deleteTM : simpl never.
+
+(** * [TrieMapLaws] *)
 
 Class TrieMapLaws (m : Type -> Type) `{TM : TrieMap m} : Prop :=
   { tml_empty {a} k :
@@ -48,7 +64,7 @@ Theorem tml_delete_there `{TML : TrieMapLaws m} {a} k (tm : m a) k' :
 Proof. by move=> NEQ; rewrite /deleteTM tml_alter_there. Qed.
 
 Instance TrieMapLaws__Map          {k} `{GHC.Base.Ord k}                        : TrieMapLaws (Data.Map.Internal.Map k).   Admitted.
-Instance TrieMapLaws__IntMap                                                    : TrieMapLaws IntMap.IntMap. Admitted.
+Instance TrieMapLaws__IntMap                                                    : TrieMapLaws IntMap.IntMap.               Admitted.
 Instance TrieMapLaws__MaybeMap     {m} `{TrieMapLaws m}                         : TrieMapLaws (MaybeMap m).                Admitted.
 Instance TrieMapLaws__ListMap      {m} `{TrieMapLaws m}                         : TrieMapLaws (ListMap m).                 Admitted.
 Instance TrieMapLaws__UniqDFM                                                   : TrieMapLaws UniqDFM.UniqDFM.             Admitted.
@@ -73,3 +89,204 @@ Instance TrieMapLaws__CoercionMapG                                              
 
 Instance TrieMapLaws__TyLitMap                                                  : TrieMapLaws TyLitMap.                    Admitted.
 
+
+(** * [TrieMap_AllKV] *)
+
+Definition TrieMap_AllKV `{TrieMap M} {A} P (m : M A) : Prop :=
+  forall k, maybe True (P k) (lookupTM k m).
+
+Theorem TrieMap_AllKV_nil `{TrieMapLaws M} {A} (P : Key M -> A -> Prop) : TrieMap_AllKV P emptyTM.
+Proof. by red=> k; rewrite tml_empty. Qed.
+
+Theorem TrieMap_AllKV_lookup_Some `{TrieMap M} {A} P (m : M A) k v :
+  TrieMap_AllKV P m ->
+  lookupTM k m = Some v ->
+  P k v.
+Proof.
+  rewrite /TrieMap_AllKV => /(_ k) ALL SOME.
+  by move: ALL; rewrite SOME.
+Qed.
+
+Theorem TrieMap_AllKV_alter_lookup `{TrieMapLaws M} {A} (P : Key M -> A -> Prop) k f m :
+  comparable (Key M) ->
+  (forall k, maybe True (P k) (lookupTM k m) -> maybe True (P k) (f (lookupTM k m))) ->
+  TrieMap_AllKV P m ->
+  TrieMap_AllKV P (alterTM k f m).
+Proof.
+  move=> dec preservation All_m.
+  red=> k'; case: (dec k k') => [<-{k'}|NEQ].
+  - rewrite tml_alter_here /=.
+    by apply preservation.
+  - by rewrite tml_alter_there.
+Qed.
+
+Theorem TrieMap_AllKV_alter `{TrieMapLaws M} {A} (P : Key M -> A -> Prop) k f m :
+  comparable (Key M) ->
+  (forall k mv, maybe True (P k) mv -> maybe True (P k) (f mv)) ->
+  TrieMap_AllKV P m ->
+  TrieMap_AllKV P (alterTM k f m).
+Proof.
+  move=> dec preservation.
+  by apply TrieMap_AllKV_alter_lookup => // k' /(preservation _).
+Qed.
+
+Theorem TrieMap_AllKV_map `{TrieMapLaws M} {A B} P (f : A -> B) (m : M A) :
+  TrieMap_AllKV P (mapTM f m) <-> TrieMap_AllKV (fun k => P k ∘ f) m.
+Proof.
+  rewrite /TrieMap_AllKV; split.
+  all: move=> Hyp k; move: {Hyp} (Hyp k).
+  all: rewrite -tml_map.
+  all: by case: (lookupTM k m).
+Qed.
+
+Theorem TrieMap_AllKV_insert `{TrieMapLaws M} {A} (P : Key M -> A -> Prop) k v m :
+  comparable (Key M) ->
+  P k v ->
+  TrieMap_AllKV P m ->
+  TrieMap_AllKV P (insertTM k v m).
+Proof.
+  move=> dec P_k_v All_m k'.
+  case: (dec k k') => [<-{k'}|NEQ].
+  - by rewrite tml_insert_here.
+  - by rewrite tml_insert_there.
+Qed.
+
+Theorem TrieMap_AllKV_delete `{TrieMapLaws M} {A} P k (m : M A) :
+  comparable (Key M) ->
+  TrieMap_AllKV P m ->
+  TrieMap_AllKV P (deleteTM k m).
+Proof. by move=> dec; apply TrieMap_AllKV_alter. Qed.
+
+Theorem TrieMap_AllKV_inv `{TrieMapLaws M} {A} P k v (m : M A) :
+  TrieMap_AllKV P (insertTM k v m) -> P k v.
+Proof. by move=> /(_ k); rewrite tml_insert_here. Qed.
+
+Theorem TrieMap_AllKV_insert_iff `{TrieMapLaws M} {A} P k v (m : M A) :
+  comparable (Key M) ->
+  TrieMap_AllKV P (insertTM k v m) <-> P k v /\ TrieMap_AllKV P (deleteTM k m).
+Proof.
+  move=> dec.
+  split.
+  - move=> All_m; split; first by apply TrieMap_AllKV_inv in All_m.
+    move=> k'; move: (All_m k').
+    case: (dec k k') => [<-{k'}|NEQ].
+    + by rewrite tml_delete_here.
+    + by rewrite tml_insert_there // tml_delete_there //.
+  - move=> [Pv All_del] k'; move: (All_del k').
+    case: (dec k k') => [<-{k'}|NEQ].
+    + by rewrite tml_insert_here.
+    + by rewrite tml_delete_there // tml_insert_there //.
+Qed.
+  
+Theorem TrieMap_AllKV_impl_lookup `{TrieMapLaws M} {A} (P Q : Key M -> A -> Prop) m :
+  (forall k v, lookupTM k m = Some v -> P k v -> Q k v) ->
+  TrieMap_AllKV P m -> TrieMap_AllKV Q m.
+Proof.
+  move=> impl All_P k.
+  move: (All_P k).
+  case def_v: (lookupTM k m) => [v|] //=.
+  by apply impl.
+Qed.
+
+Theorem TrieMap_AllKV_impl `{TrieMapLaws M} {A} (P Q : Key M -> A -> Prop) :
+  (forall k v, P k v -> Q k v) ->
+  forall m, TrieMap_AllKV P m -> TrieMap_AllKV Q m.
+Proof.
+  move=> impl m; apply TrieMap_AllKV_impl_lookup.
+  by move=> *; apply impl.
+Qed.
+
+(** * [TrieMap_All] *)
+
+Definition TrieMap_All `{TrieMap M} {A} P (m : M A) : Prop :=
+  forall k, maybe True P (lookupTM k m).
+
+Theorem TrieMap_All_AllKV `{TrieMap M} {A} P (m : M A) :
+  TrieMap_All P m <-> TrieMap_AllKV (const P) m.
+Proof. reflexivity. Qed.
+
+Theorem TrieMap_All_nil `{TrieMapLaws M} {A} (P : A -> Prop) : TrieMap_All P emptyTM.
+Proof. apply TrieMap_AllKV_nil. Qed.
+
+Theorem TrieMap_All_lookup_Some `{TrieMap M} {A} P (m : M A) k v :
+  TrieMap_All P m ->
+  lookupTM k m = Some v ->
+  P v.
+Proof. apply TrieMap_AllKV_lookup_Some. Qed.
+
+Theorem TrieMap_All_alter_lookup `{TrieMapLaws M} {A} (P : A -> Prop) k f (m : M A) :
+  comparable (Key M) ->
+  (forall k, maybe True P (lookupTM k m) -> maybe True P (f (lookupTM k m))) ->
+  TrieMap_All P m ->
+  TrieMap_All P (alterTM k f m).
+Proof. apply TrieMap_AllKV_alter_lookup. Qed.
+
+Theorem TrieMap_All_alter `{TrieMapLaws M} {A} (P : A -> Prop) k f (m : M A) :
+  comparable (Key M) ->
+  (forall mv, maybe True P mv -> maybe True P (f mv)) ->
+  TrieMap_All P m ->
+  TrieMap_All P (alterTM k f m).
+Proof. by move=> *; apply TrieMap_AllKV_alter. Qed.
+
+Theorem TrieMap_All_map `{TrieMapLaws M} {A B} P (f : A -> B) (m : M A) :
+  TrieMap_All P (mapTM f m) <-> TrieMap_All (P ∘ f) m.
+Proof. apply TrieMap_AllKV_map. Qed.
+
+Theorem TrieMap_All_fold_cons_nil `{TrieMapLaws M} {A} P (m : M A) :
+  TrieMap_All P m <-> Forall P (foldTM cons m nil).
+Proof.
+  rewrite Forall_forall; split.
+  - move=> All_m v.
+    rewrite tml_fold_in; move=> [k' def_k].
+    eapply TrieMap_All_lookup_Some; eassumption.
+  - move=> All_fold k.
+    case def_v: (lookupTM k m) => [v|] //=.
+    apply All_fold; rewrite tml_fold_in.
+    by exists k.
+Qed.
+
+Theorem TrieMap_All_insert `{TrieMapLaws M} {A} (P : A -> Prop) k v (m : M A) :
+  comparable (Key M) ->
+  P v ->
+  TrieMap_All P m ->
+  TrieMap_All P (insertTM k v m).
+Proof. by move=> *; apply TrieMap_AllKV_insert. Qed.
+
+Theorem TrieMap_All_delete `{TrieMapLaws M} {A} P k (m : M A) :
+  comparable (Key M) ->
+  TrieMap_All P m ->
+  TrieMap_All P (deleteTM k m).
+Proof. apply TrieMap_AllKV_delete. Qed.
+
+Theorem TrieMap_All_inv `{TrieMapLaws M} {A} P k v (m : M A) : 
+  TrieMap_All P (insertTM k v m) -> P v.
+Proof. apply TrieMap_AllKV_inv. Qed.
+
+Theorem TrieMap_All_insert_iff `{TrieMapLaws M} {A} P k v (m : M A) :
+  comparable (Key M) ->
+  TrieMap_All P (insertTM k v m) <-> P v /\ TrieMap_All P (deleteTM k m).
+Proof. apply TrieMap_AllKV_insert_iff. Qed.
+  
+Theorem TrieMap_All_impl_lookup `{TrieMapLaws M} {A} (P Q : A -> Prop) (m : M A) :
+  (forall k v, lookupTM k m = Some v -> P v -> Q v) ->
+  TrieMap_All P m -> TrieMap_All Q m.
+Proof. apply TrieMap_AllKV_impl_lookup. Qed.
+
+Theorem TrieMap_All_impl_lookup_exists `{TrieMapLaws M} {A} (P Q : A -> Prop) (m : M A) :
+  (forall v, (exists k, lookupTM k m = Some v) -> P v -> Q v) ->
+  TrieMap_All P m -> TrieMap_All Q m.
+Proof.
+  move=> impl. apply TrieMap_All_impl_lookup => k v def_v.
+  by apply impl; exists k.
+Qed.
+
+Theorem TrieMap_All_impl `{TrieMapLaws M} {A} (P Q : A -> Prop) :
+  (forall v, P v -> Q v) ->
+  forall m : M A, TrieMap_All P m -> TrieMap_All Q m.
+Proof. by move=> *; apply (TrieMap_AllKV_impl (const P) (const Q)). Qed.
+
+(** * hs_simpl *)
+
+Lemma Key_CoreMap : Key CoreMap = Core.Expr Core.Var.
+Proof. done. Qed.
+Hint Rewrite Key_CoreMap : hs_simpl.
